doc/coq/playground/Var.lean
@@ -1,9 +1,6 @@
 def tyenv.{u} := List (Type u)
 def assign.{u} := List (Σ a : Type u, Option a)
 
-inductive dummy.{u} : Type u :=
-| intro
-
 inductive filter.{u} : tyenv → assign → tyenv → Type (u + 1) :=
 | Filter_nil : filter [] [] []
 | Filter_cons_some A a γ σ γ' (FILTER : filter γ σ γ')
@@ -21,64 +18,54 @@ inductive value.{u} : tyenv → Type → Type (u + 1) :=
 
 def empty_var {A B} (x : var [] A) : B :=
   False.elim (
-    let convoy {γ} (x : var γ A) :
-      match γ with
+    let convoy {γ} (x : var γ A)
+    : match γ with
       | [] => False
       | _ :: _ => True
     :=
     match x with
     | .Var_hd => True.intro
-    | .Var_tl _ => True.intro
+    | .Var_tl _x_tl => True.intro
     convoy x
   )
 
 def shift_value {γ A} B (v : value γ A) : value (B :: γ) A :=
+  open var value in
   match v with
   | .Var x =>
     match γ with
     | [] => empty_var x
     | _τ :: _τl =>
       match x with
-      | .Var_hd => value.Var (var.Var_tl var.Var_hd)
-      | .Var_tl x => value.Var (var.Var_tl (var.Var_tl x))
+      | .Var_hd => Var (Var_tl Var_hd)
+      | .Var_tl x_tl => Var (Var_tl (Var_tl x_tl))
   | .Val v => value.Val v
 
 def assign_var {A} γ σ γ' (FILTER : filter γ σ γ') (x : var γ A) : value γ' A :=
+  open var value in
   match x with
   | .Var_hd =>
-    let convoy {Aγ} (FILTER' : filter Aγ σ γ') :
-      match Aγ with
-      | [] => dummy
-      | A :: _γ => value γ' A
-    :=
-      match FILTER' with
-      | .Filter_nil => dummy.intro
-      | .Filter_cons_some _A v _γ _σ _γ' _FILTER => id (value.Val v)
-      | .Filter_cons_none _A _γ _σ _γ' _FILTER => id (value.Var var.Var_hd)
-    convoy FILTER
-  | .Var_tl x =>
-    let convoy {Aγ} (FILTER' : filter Aγ σ γ') :
-      match Aγ with
-      | [] => dummy
-      | _τ :: τl => ∀ {B}, var τl B -> value γ' B
-    :=
-      match FILTER' with
-      | .Filter_nil => dummy.intro
-      | .Filter_cons_some _A _v γ_tl σ_tl γ'_tl FILTER'_tl => fun {B} x_tl =>
-        id (@assign_var B γ_tl σ_tl γ'_tl FILTER'_tl x_tl)
-      | .Filter_cons_none A' γ_tl σ_tl γ'_tl FILTER'_tl => fun {B} x_tl =>
-        id (shift_value A' (@assign_var B γ_tl σ_tl γ'_tl FILTER'_tl x_tl))
-    convoy FILTER x
+    match FILTER with
+    | .Filter_cons_some _A v _γ _σ _γ' _FILTER => Val v
+    | .Filter_cons_none _A _γ _σ _γ' _FILTER => Var Var_hd
+  | .Var_tl x_tl =>
+    match FILTER with
+    | .Filter_cons_some _A _v γ_tl σ_tl γ'_tl FILTER_tl =>
+      assign_var γ_tl σ_tl γ'_tl FILTER_tl x_tl
+    | .Filter_cons_none A_hd γ_tl σ_tl γ'_tl FILTER_tl =>
+      shift_value A_hd (assign_var γ_tl σ_tl γ'_tl FILTER_tl x_tl)
 
 def assign_value {A} γ σ γ' (FILTER : filter γ σ γ') (v : value γ A) : value γ' A :=
+  open value in
   match v with
   | .Var x => assign_var γ σ γ' FILTER x
-  | .Val v => value.Val v
+  | .Val v => Val v
 
 def id_filter γ : Σ σ, filter γ σ γ :=
+  open filter in
   match γ with
-  | [] => ⟨[], filter.Filter_nil⟩
+  | [] => ⟨[], Filter_nil⟩
   | τ :: τl =>
     let ⟨tl, FILTER⟩ := id_filter τl
-    ⟨⟨τ, none⟩ :: tl, filter.Filter_cons_none τ τl tl τl FILTER⟩
+    ⟨⟨τ, none⟩ :: tl, Filter_cons_none τ τl tl τl FILTER⟩
 
